---
keywords: Business,Business Leaders,Math and Statistics
title: Prior Probability
description: Prior likelihood, in Bayesian statistical surmising, is the likelihood of an event in light of laid out information, before empirical data is collected.
---

# Prior Probability
## What Is Prior Probability?

Prior likelihood, in Bayesian statistics, is the likelihood of an event before new data is collected. This is the best rational assessment of the likelihood of an outcome in view of the current information before an experiment is performed.

Prior likelihood can measure up to [posterior probability](/posterior-likelihood).

## Grasping Prior Probability

The prior likelihood of an event will be updated as new data or data opens up, to deliver a more accurate measure of a possible outcome. That overhauled likelihood turns into the posterior likelihood and is calculated utilizing [Bayes' theorem](/bayes-theorem). In statistical terms, the posterior likelihood is the likelihood of event A happening given that event B has happened.

### Example

For example, three acres of land have the marks A, B, and C. One section of land has reserves of oil below its surface, while the other two don't. The prior likelihood of oil being found on section of land C is 33%, or 0.333. However, assuming a drilling test is directed on section of land B, and the outcomes show that no oil is available at the location, then, at that point, the posterior likelihood of oil being found on acres An and C become 0.5, as every section of land has one out of two possibilities.

> Bayes' theorem is frequently applied to [data mining](/datamining) and [machine learning](/machine-learning).
>
## Bayes' Theorem
<span class="katex"><span class="katex-mathml"><math xmlns="http://www.w3.org/1998/Math/MathML"><semantics><mtable rowspacing="0.24999999999999992em" columnalign="right left" columnspacing="0em"><mtr><mtd><mstyle scriptlevel="0" displaystyle="true"><mrow></mrow></mstyle></mtd><mtd><mstyle scriptlevel="0" displaystyle="true"><mrow><mrow></mrow><mi>P</mi><mo stretchy="false">(</mo><mi>A</mi><mo>∣</mo><mi>B</mi><mo stretchy="false">)</mo><mtext> </mtext><mo>=</mo><mtext> </mtext><mfrac><mrow><mi>P</mi><mo stretchy="false">(</mo><mi>A</mi><mo>∩</mo><mi>B</mi><mo stretchy="false">)</mo></mrow><mrow><mi>P</mi><mo stretchy="false">(</mo><mi>B</mi><mo stretchy="false">)</mo></mrow></mfrac><mtext> </mtext><mo>=</mo><mtext> </mtext><mfrac><mrow><mi>P</mi><mo stretchy="false">(</mo><mi>A</mi><mo stretchy="false">)</mo><mtext> </mtext><mo>×</mo><mtext> </mtext><mi>P</mi><mo stretchy="false">(</mo><mi>B</mi><mo>∣</mo><mi>A</mi><mo stretchy="false">)</mo></mrow><mrow><mi>P</mi><mo stretchy="false">(</mo><mi>B</mi><mo stretchy="false">)</mo></mrow></mfrac></mrow></mstyle></mtd></mtr><mtr><mtd><mstyle scriptlevel="0" displaystyle="true"><mrow></mrow></mstyle></mtd><mtd><mstyle scriptlevel="0" displaystyle="true"><mrow><mrow></mrow><mtext mathvariant="bold">where:</mtext></mrow></mstyle></mtd></mtr><mtr><mtd><mstyle scriptlevel="0" displaystyle="true"><mrow></mrow></mstyle></mtd><mtd><mstyle scriptlevel="0" displaystyle="true"><mrow><mrow></mrow><mi>P</mi><mo stretchy="false">(</mo><mi>A</mi><mo stretchy="false">)</mo><mtext> </mtext><mo>=</mo><mtext> the prior probability of </mtext><mi>A</mi><mtext> occurring</mtext></mrow></mstyle></mtd></mtr><mtr><mtd><mstyle scriptlevel="0" displaystyle="true"><mrow></mrow></mstyle></mtd><mtd><mstyle scriptlevel="0" displaystyle="true"><mrow><mrow></mrow><mi>P</mi><mo stretchy="false">(</mo><mi>A</mi><mo>∣</mo><mi>B</mi><mo stretchy="false">)</mo><mo>=</mo><mtext> the conditional probability of </mtext><mi>A</mi></mrow></mstyle></mtd></mtr><mtr><mtd><mstyle scriptlevel="0" displaystyle="true"><mrow></mrow></mstyle></mtd><mtd><mstyle scriptlevel="0" displaystyle="true"><mrow><mrow></mrow><mspace width="2em"/><mspace width="2em"/><mspace width="1em"/><mtext>  given that </mtext><mi>B</mi><mtext> occurs</mtext></mrow></mstyle></mtd></mtr><mtr><mtd><mstyle scriptlevel="0" displaystyle="true"><mrow></mrow></mstyle></mtd><mtd><mstyle scriptlevel="0" displaystyle="true"><mrow><mrow></mrow><mi>P</mi><mo stretchy="false">(</mo><mi>B</mi><mo>∣</mo><mi>A</mi><mo stretchy="false">)</mo><mtext> </mtext><mo>=</mo><mtext> the conditional probability of </mtext><mi>B</mi></mrow></mstyle></mtd></mtr><mtr><mtd><mstyle scriptlevel="0" displaystyle="true"><mrow></mrow></mstyle></mtd><mtd><mstyle scriptlevel="0" displaystyle="true"><mrow><mrow></mrow><mspace width="2em"/><mspace width="2em"/><mspace width="1em"/><mtext>   given that </mtext><mi>A</mi><mtext> occurs</mtext></mrow></mstyle></mtd></mtr><mtr><mtd><mstyle scriptlevel="0" displaystyle="true"><mrow></mrow></mstyle></mtd><mtd><mstyle scriptlevel="0" displaystyle="true"><mrow><mrow></mrow><mi>P</mi><mo stretchy="false">(</mo><mi>B</mi><mo stretchy="false">)</mo><mtext> </mtext><mo>=</mo><mtext> the probability of </mtext><mi>B</mi><mtext> occurring</mtext></mrow></mstyle></mtd></mtr></mtable><annotation encoding="application/x-tex">\begin{aligned}&amp;P(A\mid B)\ =\ \frac{P(A\cap B)}{P(B)}\ = \ \frac{P(A)\ \times\ P(B\mid A)}{P(B)}\\&amp;\textbf{where:}\\&amp;P(A)\ =\ \text{the prior probability of }A\text{ occurring}\\&amp;P(A\mid B)=\ \text{the conditional probability of }A\\&amp;\qquad\qquad\quad\ \text{ given that }B\text{ occurs}\\&amp;P(B\mid A)\ = \ \text{the conditional probability of }B\\&amp;\qquad\qquad\quad\ \ \text{ given that }A\text{ occurs}\\&amp;P(B)\ =\ \text{the probability of }B\text{ occurring}\end{aligned}</annotation></semantics></math></span><span class="katex-html" aria-hidden="true"><span class="base"><span class="strut" style="height:13.163em;vertical-align:-6.331499999999999em;"></span><span class="mord"><span class="mtable"><span class="col-align-r"><span class="vlist-t vlist-t2"><span class="vlist-r"><span class="vlist" style="height:6.8315em;"><span style="top:-8.8315em;"><span class="pstrut" style="height:3.427em;"></span><span class="mord"></span></span><span style="top:-6.7555em;"><span class="pstrut" style="height:3.427em;"></span><span class="mord"></span></span><span style="top:-5.2555em;"><span class="pstrut" style="height:3.427em;"></span><span class="mord"></span></span><span style="top:-3.7555em;"><span class="pstrut" style="height:3.427em;"></span><span class="mord"></span></span><span style="top:-2.2555000000000005em;"><span class="pstrut" style="height:3.427em;"></span><span class="mord"></span></span><span style="top:-0.7555000000000005em;"><span class="pstrut" style="height:3.427em;"></span><span class="mord"></span></span><span style="top:0.744499999999999em;"><span class="pstrut" style="height:3.427em;"></span><span class="mord"></span></span><span style="top:2.244499999999999em;"><span class="pstrut" style="height:3.427em;"></span><span class="mord"></span></span></span><span class="vlist-s">​</span></span><span class="vlist-r"><span class="vlist" style="height:6.331499999999999em;"><span></span></span></span></span></span><span class="col-align-l"><span class="vlist-t vlist-t2"><span class="vlist-r"><span class="vlist" style="height:6.8315em;"><span style="top:-8.8315em;"><span class="pstrut" style="height:3.427em;"></span><span class="mord"><span class="mord"></span><span class="mord mathnormal" style="margin-right:0.13889em;">P</span><span class="mopen">(</span><span class="mord mathnormal">A</span><span class="mspace" style="margin-right:0.2777777777777778em;"></span><span class="mrel">∣</span><span class="mspace" style="margin-right:0.2777777777777778em;"></span><span class="mord mathnormal" style="margin-right:0.05017em;">B</span><span class="mclose">)</span><span class="mspace"> </span><span class="mspace" style="margin-right:0.2777777777777778em;"></span><span class="mrel">=</span><span class="mspace"> </span><span class="mspace" style="margin-right:0.2777777777777778em;"></span><span class="mord"><span class="mopen nulldelimiter"></span><span class="mfrac"><span class="vlist-t vlist-t2"><span class="vlist-r"><span class="vlist" style="height:1.427em;"><span style="top:-2.314em;"><span class="pstrut" style="height:3em;"></span><span class="mord"><span class="mord mathnormal" style="margin-right:0.13889em;">P</span><span class="mopen">(</span><span class="mord mathnormal" style="margin-right:0.05017em;">B</span><span class="mclose">)</span></span></span><span style="top:-3.23em;"><span class="pstrut" style="height:3em;"></span><span class="frac-line" style="border-bottom-width:0.04em;"></span></span><span style="top:-3.677em;"><span class="pstrut" style="height:3em;"></span><span class="mord"><span class="mord mathnormal" style="margin-right:0.13889em;">P</span><span class="mopen">(</span><span class="mord mathnormal">A</span><span class="mspace" style="margin-right:0.2222222222222222em;"></span><span class="mbin">∩</span><span class="mspace" style="margin-right:0.2222222222222222em;"></span><span class="mord mathnormal" style="margin-right:0.05017em;">B</span><span class="mclose">)</span></span></span></span><span class="vlist-s">​</span></span><span class="vlist-r"><span class="vlist" style="height:0.936em;"><span></span></span></span></span></span><span class="mclose nulldelimiter"></span></span><span class="mspace"> </span><span class="mspace" style="margin-right:0.2777777777777778em;"></span><span class="mrel">=</span><span class="mspace"> </span><span class="mspace" style="margin-right:0.2777777777777778em;"></span><span class="mord"><span class="mopen nulldelimiter"></span><span class="mfrac"><span class="vlist-t vlist-t2"><span class="vlist-r"><span class="vlist" style="height:1.427em;"><span style="top:-2.314em;"><span class="pstrut" style="height:3em;"></span><span class="mord"><span class="mord mathnormal" style="margin-right:0.13889em;">P</span><span class="mopen">(</span><span class="mord mathnormal" style="margin-right:0.05017em;">B</span><span class="mclose">)</span></span></span><span style="top:-3.23em;"><span class="pstrut" style="height:3em;"></span><span class="frac-line" style="border-bottom-width:0.04em;"></span></span><span style="top:-3.677em;"><span class="pstrut" style="height:3em;"></span><span class="mord"><span class="mord mathnormal" style="margin-right:0.13889em;">P</span><span class="mopen">(</span><span class="mord mathnormal">A</span><span class="mclose">)</span><span class="mspace"> </span><span class="mspace" style="margin-right:0.2222222222222222em;"></span><span class="mbin">×</span><span class="mspace"> </span><span class="mspace" style="margin-right:0.2222222222222222em;"></span><span class="mord mathnormal" style="margin-right:0.13889em;">P</span><span class="mopen">(</span><span class="mord mathnormal" style="margin-right:0.05017em;">B</span><span class="mspace" style="margin-right:0.2777777777777778em;"></span><span class="mrel">∣</span><span class="mspace" style="margin-right:0.2777777777777778em;"></span><span class="mord mathnormal">A</span><span class="mclose">)</span></span></span></span><span class="vlist-s">​</span></span><span class="vlist-r"><span class="vlist" style="height:0.936em;"><span></span></span></span></span></span><span class="mclose nulldelimiter"></span></span></span></span><span style="top:-6.7555em;"><span class="pstrut" style="height:3.427em;"></span><span class="mord"><span class="mord"></span><span class="mord text"><span class="mord textbf">where:</span></span></span></span><span style="top:-5.2555em;"><span class="pstrut" style="height:3.427em;"></span><span class="mord"><span class="mord"></span><span class="mord mathnormal" style="margin-right:0.13889em;">P</span><span class="mopen">(</span><span class="mord mathnormal">A</span><span class="mclose">)</span><span class="mspace"> </span><span class="mspace" style="margin-right:0.2777777777777778em;"></span><span class="mrel">=</span><span class="mspace"> </span><span class="mspace" style="margin-right:0.2777777777777778em;"></span><span class="mord text"><span class="mord">the prior probability of </span></span><span class="mord mathnormal">A</span><span class="mord text"><span class="mord"> occurring</span></span></span></span><span style="top:-3.7555em;"><span class="pstrut" style="height:3.427em;"></span><span class="mord"><span class="mord"></span><span class="mord mathnormal" style="margin-right:0.13889em;">P</span><span class="mopen">(</span><span class="mord mathnormal">A</span><span class="mspace" style="margin-right:0.2777777777777778em;"></span><span class="mrel">∣</span><span class="mspace" style="margin-right:0.2777777777777778em;"></span><span class="mord mathnormal" style="margin-right:0.05017em;">B</span><span class="mclose">)</span><span class="mspace" style="margin-right:0.2777777777777778em;"></span><span class="mrel">=</span><span class="mspace"> </span><span class="mspace" style="margin-right:0.2777777777777778em;"></span><span class="mord text"><span class="mord">the conditional probability of </span></span><span class="mord mathnormal">A</span></span></span><span style="top:-2.2555000000000005em;"><span class="pstrut" style="height:3.427em;"></span><span class="mord"><span class="mord"></span><span class="mspace" style="margin-right:2em;"></span><span class="mspace" style="margin-right:2em;"></span><span class="mspace" style="margin-right:1em;"></span><span class="mspace"> </span><span class="mord text"><span class="mord"> given that </span></span><span class="mord mathnormal" style="margin-right:0.05017em;">B</span><span class="mord text"><span class="mord"> occurs</span></span></span></span><span style="top:-0.7555000000000005em;"><span class="pstrut" style="height:3.427em;"></span><span class="mord"><span class="mord"></span><span class="mord mathnormal" style="margin-right:0.13889em;">P</span><span class="mopen">(</span><span class="mord mathnormal" style="margin-right:0.05017em;">B</span><span class="mspace" style="margin-right:0.2777777777777778em;"></span><span class="mrel">∣</span><span class="mspace" style="margin-right:0.2777777777777778em;"></span><span class="mord mathnormal">A</span><span class="mclose">)</span><span class="mspace"> </span><span class="mspace" style="margin-right:0.2777777777777778em;"></span><span class="mrel">=</span><span class="mspace"> </span><span class="mspace" style="margin-right:0.2777777777777778em;"></span><span class="mord text"><span class="mord">the conditional probability of </span></span><span class="mord mathnormal" style="margin-right:0.05017em;">B</span></span></span><span style="top:0.744499999999999em;"><span class="pstrut" style="height:3.427em;"></span><span class="mord"><span class="mord"></span><span class="mspace" style="margin-right:2em;"></span><span class="mspace" style="margin-right:2em;"></span><span class="mspace" style="margin-right:1em;"></span><span class="mspace"> </span><span class="mspace"> </span><span class="mord text"><span class="mord"> given that </span></span><span class="mord mathnormal">A</span><span class="mord text"><span class="mord"> occurs</span></span></span></span><span style="top:2.244499999999999em;"><span class="pstrut" style="height:3.427em;"></span><span class="mord"><span class="mord"></span><span class="mord mathnormal" style="margin-right:0.13889em;">P</span><span class="mopen">(</span><span class="mord mathnormal" style="margin-right:0.05017em;">B</span><span class="mclose">)</span><span class="mspace"> </span><span class="mspace" style="margin-right:0.2777777777777778em;"></span><span class="mrel">=</span><span class="mspace"> </span><span class="mspace" style="margin-right:0.2777777777777778em;"></span><span class="mord text"><span class="mord">the probability of </span></span><span class="mord mathnormal" style="margin-right:0.05017em;">B</span><span class="mord text"><span class="mord"> occurring</span></span></span></span></span><span class="vlist-s">​</span></span><span class="vlist-r"><span class="vlist" style="height:6.331499999999999em;"><span></span></span></span></span></span></span></span></span></span></span>
Assuming we are keen on the likelihood of an event of which we have prior perceptions; we call this the prior likelihood. We'll consider this event A, and its likelihood P(A). In the event that there is a second event that influences P(A), which we'll call event B, then we need to understand what the likelihood of An is given B has happened. In probabilistic documentation, this is P(A|B), and is known as posterior likelihood or changed likelihood. This is on the grounds that it has happened after the original event, subsequently the post in posterior. This is the way Baye's theorem extraordinarily permits us to refresh our previous convictions with new data.

## Features
- In statistical terms, the prior likelihood is the basis for posterior probabilities.
- A prior likelihood, in Bayesian statistics, is the ex-ante probability of an event happening before thinking about any new (posterior) data.
- The posterior likelihood is calculated by refreshing the prior likelihood utilizing Bayes' theorem.
## FAQ
### How Is Bayes' Theorem Used in Machine Learning?
Bayes Theorem gives a valuable method to contemplating the relationship between a data set and a likelihood. It is hence helpful in fitting data and training calculations, where these are able to refresh their posterior probabilities given each round of training.
### What Is the Difference Between Prior and Posterior Probability?
Prior likelihood addresses what is originally accepted before new evidence is presented, and posterior likelihood considers this new data.
### How Is Bayes' Theorem Used in Finance?
In finance, Bayes' theorem can be utilized to refresh a previous conviction once new data is gotten. This can be applied to stock returns, noticed volatility, etc. Bayes' Theorem can likewise be utilized to rate the gamble of lending money to expected borrowers by refreshing the probability of default in view of past experience.
